Checkpoint minor MkTxn progress

src/program_proof/txn/recovery_proof.v
@@ -11,19 +11,58 @@ From Perennial.goose_lang.lib Require Import slice.typed_slice.
 Section goose_lang.
 Context `{!txnG Σ}.
 
-(* TODO: set up crash_obligation_alt for txn *)
-
 (* Definitely missing the durable invariant of the heapspec layer, which should
 say something more complete about [γ.(txn_walnames)]. Otherwise there probably
 isn't enough to relate the state inside [is_txn_always] to that in
 [is_wal_inner_durable]. *)
-Theorem wp_MkTxn (d:loc) σ dinit (γ:txn_names) :
-  {{{ is_wal_inner_durable γ.(txn_walnames).(wal_heap_walnames) σ dinit ∗
-      is_txn_always γ
-  }}}
-    MkTxn #d
-  {{{ (l: loc) (γ':txn_names), RET #l; is_txn l γ' dinit }}}.
+
+Definition is_txn_durable γ dinit : iProp Σ :=
+  ∃ ls',
+  "His_wal_inner_durable" ∷ is_wal_inner_durable γ.(txn_walnames).(wal_heap_walnames) ls' dinit ∗
+  "Hwal_res" ∷ wal_resources γ.(txn_walnames).(wal_heap_walnames) ∗
+  "Hwal_heap_inv" ∷ wal_heap_inv γ.(txn_walnames) ls' ∗
+  "Hlocked_walheap" ∷ is_locked_walheap γ.(txn_walnames) {| locked_wh_σd := ls'.(log_state.d);
+                        locked_wh_σtxns := ls'.(log_state.txns);
+                    |} ∗
+  "His_txn_always" ∷ is_txn_always γ ∗
+  ∃ crash_heaps,
+  (* ⌜ lb < length ls'.(log_state.txns) ⌝%nat ∗ *)
+  "Hcrash_heaps" ∷ ghost_var γ.(txn_walnames).(wal_heap_crash_heaps) (3/4) crash_heaps ∗
+  "Hgh_ptsto" ∷ ([∗ map] a↦b ∈ latest crash_heaps, ∃ hb,
+    ⌜hb_latest_update hb = b⌝ ∗
+    mapsto (hG:=γ.(txn_walnames).(wal_heap_h)) a 1 hb).
+
+Definition txn_exchanger (γ γ' : @txn_names Σ) : iProp Σ := True.
+
+Instance is_txn_durable_discretizable γ dinit :
+  Discretizable (is_txn_durable γ dinit).
+Proof. admit. Admitted.
+
+Theorem wpc_MkTxn (d:loc) dinit (γ:txn_names) logm k :
+  {{{ is_txn_durable γ dinit ∗ ghost_var γ.(txn_crashstates) (3/4) logm }}}
+    MkTxn #d @ NotStuck; k; ⊤
+  {{{ (l: loc), RET #l; is_txn l γ dinit ∗ ([∗ map] a ↦ v ∈ latest (logm), mapsto_txn γ a v)
+      (* cfupd stuff *) }}}
+  {{{ ∃ γ', ⌜ txn_kinds γ' = txn_kinds γ ⌝ ∗ is_txn_durable γ' dinit ∗ txn_exchanger γ γ' }}}.
 Proof.
+  iIntros (Φ Φc) "(Hdur&Hlogm) HΦ".
+  rewrite /MkTxn. wpc_pures.
+  { crash_case. iNext. iExists γ. iSplit; first done. iFrame "Hdur". }
+
+  iCache with "Hdur HΦ Hlogm".
+  { crash_case.  iExists γ. iSplit; first done. iFrame "Hdur". }
+  wpc_bind (lock.new _).
+  wpc_frame; wp_apply (wp_new_free_lock).
+  iIntros (lk) "Hlock". iNamed 1.
+  wpc_bind (MkLog #d).
+  iNamed "Hdur".
+  iMod (alloc_heapspec_init_ghost_state (γ.(txn_walnames).(wal_heap_walnames)))
+         as (γ'_txn_walnames ?) "Hheapspec_init_ghost_state".
+  set (P := λ ls, (wal_heap_inv γ.(txn_walnames) ls ∗ heapspec_init_ghost_state γ'_txn_walnames)%I).
+  (* TODO: need init_ghost_state for the txn so we can define γ', the new names *)
+  set (Prec := True).
+  set (Pcrash := True).
+  wpc_apply (wpc_MkLog_recover dinit P).
 Admitted.
 
 End goose_lang.
